

In this section we work out explicitly the reduction of the exact N interacting Fermion Hamiltonian to a reduced “complete active space” of orbitals. That is, beginning from the second-quantized interacting Hamiltonian

$$H = \sum_{ij} h_{ij} a_i^\dagger a_j + \frac{1}{2} h_{ijkl} a_i^\dagger a_j^\dagger a_k a_l, \quad (1)$$

we will assume that some index set  $\mathcal{I}_C$  is now fully occupied, or is the frozen “core” and some index set  $\mathcal{I}_V$  is totally unoccupied, or virtual. The active set of orbitals belongs to the index set  $\mathcal{I}_A$ . All Hamiltonians here will assume the integrals have been worked out in the spin-orbital basis so as to include the spin properly. We will denote the total number of spin-orbitals/sites to be  $M$  and total number of fermions to be  $N_e$ . Without loss of generality we will order the orbitals such that the first  $N_e$  orbitals are frozen. Under this convention, all wavefunctions in the active space may be written as

$$|\Psi\rangle = \prod_{j=N_c+1}^N \left( \sum_{k=N_c+1}^M c_k^j a_j^\dagger \right) \prod_{\lambda=1}^{N_c} a_\lambda^\dagger | \rangle \quad (2)$$

where the product operator is assumed to fill from the right, e.g.  $\prod_{\lambda=1}^2 a_\lambda^\dagger = a_2^\dagger a_1^\dagger$ . Thus to find a Hamiltonian with equivalent action on the active space under the assumption of filled core orbitals, we examine the action of the dressed Hamiltonian on the resulting subsystem of  $N - N_c$  electrons in  $M - N_c$  orbitals which is given by

$$\tilde{H} = \left( \prod_{\lambda=N_c}^1 a_\lambda \right) H \left( \prod_{\lambda=1}^{N_c} a_\lambda^\dagger \right). \quad (3)$$

To proceed, it will be useful to work out the dressing for a single term for both the 1- and 2-fermion operators, which after copious use of Wick’s theorem and an assumption that the index  $\lambda$  will not

appear in the remaining wavefunction, turn out to be

$$ca_\lambda a_\lambda^\dagger = c \quad (4)$$

$$a_\lambda h_{ij} a_i^\dagger a_j a_\lambda^\dagger = h_{ij} \left[ a_i^\dagger a_j + \delta_{\lambda i} \delta_{j\lambda} \right] \quad (5)$$

$$\begin{aligned} a_\lambda h_{ijkl} a_i^\dagger a_j^\dagger a_k a_l a_\lambda^\dagger &= h_{ijkl} \left[ a_i^\dagger a_j^\dagger a_k a_l \right. \\ &\quad - \delta_{\lambda i} \delta_{k\lambda} a_j^\dagger a_l + \delta_{\lambda i} \delta_{l\lambda} a_j^\dagger a_k \\ &\quad \left. + \delta_{\lambda j} \delta_{k\lambda} a_i^\dagger a_l - \delta_{\lambda j} \delta_{l\lambda} a_i^\dagger a_k \right] \end{aligned} \quad (6)$$

where  $c$  is any generic constant. The form of these terms allows one to extend by induction to a dressing of all  $N_c$  terms with the same assumptions, which yields

$$c \prod_\lambda a_\lambda \prod_\lambda a_\lambda^\dagger = c \quad (7)$$

$$\begin{aligned} \prod_\lambda a_\lambda h_{ij} a_i^\dagger a_j \prod_\lambda a_\lambda^\dagger &= h_{ij} \left[ a_i^\dagger a_j + \sum_\lambda \delta_{\lambda i} \delta_{j\lambda} \right] \quad (8) \\ \prod_\lambda a_\lambda h_{ijkl} a_i^\dagger a_j^\dagger a_k a_l \prod_\lambda a_\lambda^\dagger &= h_{ijkl} \left[ a_i^\dagger a_j^\dagger a_k a_l \right. \\ &\quad + \sum_\lambda \left( -\delta_{\lambda i} \delta_{k\lambda} a_j^\dagger a_l + \delta_{\lambda i} \delta_{l\lambda} a_j^\dagger a_k \right. \\ &\quad \left. \left. + \delta_{\lambda j} \delta_{k\lambda} a_i^\dagger a_l - \delta_{\lambda j} \delta_{l\lambda} a_i^\dagger a_k \right) \right. \\ &\quad + \sum_{\lambda\sigma} \left( -\delta_{\lambda i} \delta_{k\lambda} \delta_{\sigma j} \delta_{l\sigma} + \delta_{\lambda i} \delta_{l\lambda} \delta_{\sigma j} \delta_{k\sigma} \right. \\ &\quad \left. \left. + \delta_{\lambda j} \delta_{k\lambda} \delta_{\sigma i} \delta_{l\sigma} - \delta_{\lambda j} \delta_{l\lambda} \delta_{\sigma i} \delta_{k\sigma} \right) \right]. \end{aligned}$$

Regrouping these terms by the number of fermions they act on and using the symmetry of the

two-fermion integrals in physicist notation, we arrive at the Hamiltonian which takes the form

$$H_{\text{core}} = \sum_{\lambda} h_{\lambda\lambda} + \frac{1}{2} \sum_{\lambda\sigma} -h_{\lambda\sigma\lambda\sigma} + h_{\lambda\sigma\sigma\lambda} + h_{\sigma\lambda\lambda\sigma} - h_{\sigma\lambda\sigma\lambda} \quad (9)$$

$$= \sum_{\lambda} h_{\lambda\lambda} + \sum_{\lambda\sigma} (h_{\lambda\sigma\sigma\lambda} - h_{\lambda\sigma\lambda\sigma}) \quad (10)$$

$$H_{\text{one}} = \sum_{ij} \left[ h_{ij} + \sum_{\lambda} (h_{\lambda ij\lambda} - h_{\lambda i\lambda j}) \right] a_i^{\dagger} a_j \quad (11)$$

$$H_{\text{two}} = \frac{1}{2} \sum_{ijkl} h_{ijkl} a_i^{\dagger} a_j^{\dagger} a_k a_l \quad (12)$$

$$H = H_{\text{core}} + H_{\text{one}} + H_{\text{two}}. \quad (13)$$

The assumption of unoccupied virtual states enters as a trivial restriction of the range of the sums in the operators. As a result, the new Hamiltonian operator acts only on sites from  $N_c + 1$  to  $N - N_v - 1$ , and has at most  $N_e$  electrons in it. The simplest way to summarize this result is by defining the transformed active space Hamiltonian with its new effective coefficients

$$\tilde{H} = \sum_{ij \in \mathcal{I}_A} \tilde{h}_{ij} a_i^{\dagger} a_j + \sum_{ijkl \in \mathcal{I}_A} \tilde{h}_{ijkl} a_i^{\dagger} a_j^{\dagger} a_k a_l + \tilde{C} \quad (14)$$

$$\tilde{C} = \sum_{\lambda \in \mathcal{I}_C} h_{\lambda\lambda} + \sum_{\lambda\sigma \in \mathcal{I}_C} (h_{\lambda\sigma\sigma\lambda} - h_{\lambda\sigma\lambda\sigma}) \quad (15)$$

$$\tilde{h}_{ij} = h_{ij} + \sum_{\lambda \in \mathcal{I}_C} (h_{\lambda ij\lambda} - h_{\lambda i\lambda j}) \quad (16)$$

$$\tilde{h}_{ijkl} = h_{ijkl} \quad (17)$$